max-n-sum.dfy
@@ -1,4 +1,5 @@
 ﻿/**
+ * Source:
  * http://www.lexicalscope.com/blog/2015/04/10/dafny-sum-and-max-solution/
  */
 
